theories/Rad.v
@@ -3491,7 +3491,7 @@ Module Misra(Name : UsualDecidableSet)(NetModF : NET).
       exists n1, dep_on N n0 n1 /\ dep_on N n1 n1.
 
     Proof with eattac.
-      intros HSRPC Hd.
+      intros BSRPC Hd.
 
       assert (forall n, AnySRPC_pq (NetMod.get n N)) as Hsrpc by eauto with LTS.
 
